Cleaning up: merge Inline/InlineFacts

src/InlineFacts.v
@@ -5,6 +5,8 @@ Require Import Syntax Semantics SemFacts Refinement Wf Inline.
 
 Require Import FunctionalExtensionality.
 
+Set Implicit Arguments.
+
 Lemma inlineDm_SemAction_intact:
   forall {retK} or a nr calls (retV: type retK),
     SemAction or a nr calls retV ->
@@ -566,7 +568,7 @@ Proof.
   intros; unfold inlineDms.
   remember (namesOf (getDefsBodies m)) as dms; clear Heqdms.
   generalize dependent m; induction dms; intros; [assumption|]; simpl.
-  pose proof (inlineDmToMod_wellHidden m l a H) as iwh.
+  pose proof (inlineDmToMod_wellHidden a H) as iwh.
   simpl; remember (inlineDmToMod m a) as imb; destruct imb; simpl in *.
   pose proof (IHdms _ iwh) as sth.
   remember (inlineDms' m0 dms) as imb'; destruct imb'; simpl in *.
@@ -1118,9 +1120,9 @@ Proof.
   destruct imc; [|inv Hin].
   assert (Hit: snd (inline m) = true)
     by (rewrite <-Heqimb; inv Hin; auto).
-  pose proof (inline_correct_Step _ Hequiv Hdms Hit _ _ _ H).
+  pose proof (inline_correct_Step Hequiv Hdms Hit H).
   rewrite <-Heqimb in H0; simpl in H0.
-  pose proof (step_dms_hidden _ _ _ _ H).
+  pose proof (step_dms_hidden H).
   apply step_dms_weakening; auto.
   - replace im with (fst (inline m)) by (rewrite <-Heqimb; auto).
     apply inline_ModEquiv; auto.
@@ -1199,4 +1201,735 @@ Proof.
   - apply inlineF_refines; auto.
   - auto.
 Qed.
+
+
+(** Now for fine-grained partial inlining *)
+Section NoCallDmSig.
+  Fixpoint noCallDmSigA {retT} (a: ActionT typeUT retT) (dmn: string) (dsig: SignatureT) :=
+    match a with
+    | MCall name sig _ cont =>
+      ((negb (string_eq name dmn))
+       || (if SignatureT_dec sig dsig then false else true))
+        && (noCallDmSigA (cont tt) dmn dsig)
+    | Let_ _ ar cont => noCallDmSigA (cont (getUT _)) dmn dsig
+    | ReadReg reg k cont => noCallDmSigA (cont (getUT _)) dmn dsig
+    | WriteReg reg _ e cont => noCallDmSigA cont dmn dsig
+    | IfElse ce _ ta fa cont =>
+      (noCallDmSigA ta dmn dsig) && (noCallDmSigA fa dmn dsig) && (noCallDmSigA (cont tt) dmn dsig)
+    | Assert_ ae cont => noCallDmSigA cont dmn dsig
+    | Return e => true
+    end.
+
+  Definition noCallDmSigDms (dms: list DefMethT) (ndm: DefMethT) :=
+    Forall (fun dm: DefMethT =>
+              noCallDmSigA (projT2 (attrType dm) typeUT tt) (attrName ndm)
+                           (projT1 (attrType ndm)) = true) dms.
+
+  Definition noCallDmSigRules (rules: list (Attribute (Action Void))) (ndm: DefMethT) :=
+    Forall (fun r: Attribute (Action Void) =>
+              noCallDmSigA (attrType r typeUT) (attrName ndm)
+                           (projT1 (attrType ndm)) = true) rules.
+
+  Definition noCallDmSig (m: Modules) (ndm: DefMethT) :=
+    (noCallDmSigRules (getRules m) ndm) /\ (noCallDmSigDms (getDefsBodies m) ndm).
+
+End NoCallDmSig.
+
+Lemma noCallDmSigA_semAction_calls:
+  forall {retK} (aty: ActionT type retK) aut (Hequiv: ActionEquiv aty aut)
+         (dm: DefMethT),
+    noCallDmSigA aut (attrName dm) (projT1 (attrType dm)) = true ->
+    forall s o u cs retv,
+      SemAction o aty u cs retv ->
+      Some s = M.find (attrName dm) cs ->
+      projT1 s = projT1 (attrType dm) ->
+      False.
+Proof.
+  induction 1; simpl; intros; auto.
+
+  - inv H2; destruct_existT.
+    apply andb_true_iff in H1; dest.
+    remember (string_eq n (attrName dm)) as ndeq; destruct ndeq.
+    + apply string_eq_dec_eq in Heqndeq; subst; mred.
+      simpl in H4; clear -H1 H4; subst.
+      destruct (SignatureT_dec _ _); auto.
+      discriminate.
+    + apply string_eq_dec_neq in Heqndeq.
+      rewrite M.find_add_2 in H3 by intuition.
+      eapply H0; eauto.
+
+  - inv H2; destruct_existT; eapply H0; eauto.
+  - inv H2; destruct_existT; eapply H0; eauto.
+  - inv H0; destruct_existT; eapply IHHequiv; eauto.
+  - apply andb_true_iff in H1; dest.
+    apply andb_true_iff in H1; dest.
+    inv H2; destruct_existT.
+    + rewrite M.find_union in H3.
+      remember (M.find (attrName dm) calls1) as odc1; destruct odc1.
+      * inv H3; eapply IHHequiv1; eauto.
+      * eapply H0; eauto.
+    + rewrite M.find_union in H3.
+      remember (M.find (attrName dm) calls1) as odc1; destruct odc1.
+      * inv H3; eapply IHHequiv2; eauto.
+      * eapply H0; eauto.
+  - inv H0; destruct_existT; eapply IHHequiv; eauto.
+  - inv H0; destruct_existT; mred.
+Qed.
+
+Lemma appendAction_noCallDmSigA:
+  forall {retK1 retK2} (a1: ActionT typeUT retK1)
+         (a2: typeUT retK1 -> ActionT typeUT retK2) dmn dsig,
+    noCallDmSigA (appendAction a1 a2) dmn dsig =
+    noCallDmSigA a1 dmn dsig && noCallDmSigA (a2 tt) dmn dsig.
+Proof.
+  induction a1; simpl; intros; auto.
+  - rewrite <-andb_assoc; f_equal; auto.
+  - do 3 rewrite <-andb_assoc; repeat f_equal; auto.
+Qed.
+
+Lemma noCallDm_noCallDmSigA:
+  forall tdm dm,
+    noCallDm tdm dm = true ->
+    noCallDmSigA (projT2 (attrType tdm) typeUT tt)
+                 (attrName dm) (projT1 (attrType dm)) = true.
+Proof.
+  unfold noCallDm; intros.
+  generalize dependent (projT2 (attrType tdm) typeUT tt).
+  clear; intros.
+  induction a; simpl; intros; auto; simpl in *.
+  - apply andb_true_iff in H; dest.
+    apply andb_true_iff; split; auto.
+    remember (string_eq meth (attrName dm)) as md; destruct md.
+    + apply string_eq_dec_eq in Heqmd; subst.
+      exfalso; rewrite string_eq_true in H.
+      inv H.
+    + auto.
+  - apply andb_true_iff in H; dest.
+    apply andb_true_iff in H; dest.
+    apply andb_true_iff; split; auto.
+    apply andb_true_iff; split; auto.
+Qed.
+
+Lemma noCalls_noCallDmSigATrue:
+  forall k (a: ActionT typeUT k) dmName dmBody,
+    ~ In dmName (getCallsA a) -> noCallDmSigA a dmName dmBody = true.
+Proof.
+  induction a; simpl in *; auto; intros.
+  - assert (sth1: meth <> dmName) by intuition auto.
+    assert (sth2: ~ In dmName (getCallsA (a tt))) by intuition auto.
+    unfold negb, orb, andb.
+    case_eq (string_eq meth dmName); intros.
+    + apply eq_sym in H1; apply string_eq_dec_eq in H1; subst; intuition.
+    + apply H; auto.
+  - rewrite IHa1, IHa2, H; auto; unfold not; intros.
+    + assert (In dmName (getCallsA a1 ++ getCallsA a2 ++ getCallsA (a3 tt)))
+        by (apply in_or_app; right; apply in_or_app; right; intuition auto).
+      auto.
+    + assert (In dmName (getCallsA a1 ++ getCallsA a2 ++ getCallsA (a3 tt)))
+        by (apply in_or_app; right; apply in_or_app; left; intuition auto).
+      auto.
+    + assert (In dmName (getCallsA a1 ++ getCallsA a2 ++ getCallsA (a3 tt)))
+        by (apply in_or_app; left; intuition auto).
+      auto.
+Qed.
+
+Lemma inlineDm_noCallDmSigA:
+  forall (dm: DefMethT)
+         (Hdm: noCallDmSigA (projT2 (attrType dm) typeUT tt)
+                            (attrName dm) (projT1 (attrType dm)) = true)
+         {retK} (a: ActionT typeUT retK),
+    noCallDmSigA (inlineDm a dm) (attrName dm) (projT1 (attrType dm)) = true.
+Proof.
+  induction a; simpl; intros; auto;
+    [|do 2 (apply andb_true_iff; split; auto)].
+
+  unfold getBody.
+  remember (string_eq meth (attrName dm)) as md; destruct md;
+    [|simpl; rewrite <-Heqmd; simpl; auto].
+  destruct (SignatureT_dec _ _).
+  - simpl; rewrite appendAction_noCallDmSigA.
+    apply andb_true_iff; split; auto.
+    subst; simpl.
+    assumption.
+  - simpl; rewrite <-Heqmd; simpl.
+    destruct (SignatureT_dec _ _); [elim n; auto|].
+    simpl; auto.
+Qed.
+
+Lemma inlineDmToRule_noCallDmSigA:
+  forall (dm: DefMethT)
+         (Hdm: noCallDmSigA (projT2 (attrType dm) typeUT tt)
+                            (attrName dm) (projT1 (attrType dm)) = true) r,
+    noCallDmSigA (attrType (inlineDmToRule r dm) typeUT)
+                 (attrName dm) (projT1 (attrType dm)) = true.
+Proof.
+  intros; apply inlineDm_noCallDmSigA; auto.
+Qed.
+
+Lemma noCallDmSig_substep_calls:
+  forall m o u ul cs,
+    ModEquiv type typeUT m ->
+    Substep m o u ul cs ->
+    forall dm s,
+      noCallDmSig m dm ->
+      Some s = M.find (elt:=sigT SignT) (attrName dm) cs ->
+      projT1 s = projT1 (attrType dm) ->
+      False.
+Proof.
+  intros; inv H0; try (mred; fail).
+
+  - inv H; rewrite RulesEquiv_in in H0.
+    specialize (H0 _ HInRules); unfold RuleEquiv in H0; simpl in H0.
+    unfold noCallDmSig in H1; dest.
+    unfold noCallDmSigRules in H; rewrite Forall_forall in H.
+    specialize (H _ HInRules); simpl in H.
+    eapply noCallDmSigA_semAction_calls; eauto.
+
+  - inv H; rewrite MethsEquiv_in in H4.
+    specialize (H4 _ HIn); unfold MethEquiv in H4; simpl in H4.
+    unfold noCallDmSig in H1; dest.
+    unfold noCallDmSigDms in H1; rewrite Forall_forall in H1.
+    specialize (H1 _ HIn); simpl in H1.
+    eapply noCallDmSigA_semAction_calls; eauto.
+Qed.
+
+Lemma noCallDmSig_substepsInd_calls:
+  forall m o u l,
+    ModEquiv type typeUT m ->
+    SubstepsInd m o u l ->
+    forall dm s,
+      noCallDmSig m dm ->
+      Some s = M.find (elt:=sigT SignT) (attrName dm) (calls l) ->
+      projT1 s = projT1 (attrType dm) ->
+      False.
+Proof.
+  induction 2; simpl; intros; [mred|].
+  subst; destruct l as [ann ds cs]; simpl in *.
+  rewrite M.find_union in H6.
+  remember (M.find (attrName dm) scs) as odsc; destruct odsc.
+  - inv H6; apply noCallDmSig_substep_calls with (dm:= dm) (s:= s0) in H1; auto.
+  - eapply IHSubstepsInd; eauto.
+Qed.
+
+Lemma stepInd_filterDm:
+  forall regs rules dms o u l,
+    ModEquiv type typeUT (Mod regs rules dms) ->
+    NoDup (getDefs (Mod regs rules dms)) ->
+    StepInd (Mod regs rules dms) o u l ->
+    forall (dm: DefMethT),
+      In dm dms ->
+      M.find (attrName dm) (defs l) = None ->
+      noCallDmSig (Mod regs rules dms) dm ->
+      StepInd (Mod regs rules (filterDm dms (attrName dm))) o u l.
+Proof.
+  intros; inv H1; constructor; [|apply filterDm_wellHidden; auto].
+
+  remember (M.find (attrName dm) (defs l0)) as odl; destruct odl.
+
+  - pose proof (substepsInd_defs_sig _ H0 H2 HSubSteps Heqodl).
+    remember (M.find (attrName dm) (calls l0)) as ocl; destruct ocl.
+
+    + assert (s = s0); subst.
+      { clear -H3 Heqodl Heqocl.
+        destruct l0 as [ann ds cs]; simpl in *.
+        findeq.
+      }
+      exfalso; eapply noCallDmSig_substepsInd_calls; eauto.
+
+    + exfalso; clear -H3 Heqodl Heqocl.
+      destruct l0 as [ann ds cs]; simpl in *.
+      findeq.
+
+  - assert (None = M.find (attrName dm) (calls l0)).
+    { apply wellHidden_find_1 with (a:= attrName dm) in HWellHidden.
+      { destruct HWellHidden; auto.
+        rewrite Heqodl; auto.
+      }
+      { simpl; apply in_map; auto. }
+    }
+    apply substepsInd_dm_weakening; auto.
+Qed.
+
+(* Partial inlining interfaces *)
+Section Partial.
+  Variable m: Modules.
+
+  Variable dm: DefMethT. (* a method to be inlined *)
+  Hypotheses (Hdm: In dm (getDefsBodies m))
+             (HnoDupMeths: NoDup (namesOf (getDefsBodies m))).
+  Variable r: Attribute (Action Void). (* a rule calling dm *)
+  Hypothesis Hrule: In r (getRules m).
+
+  Lemma inlineDmToRule_substepsInd_intact_1:
+    forall o u l,
+      SubstepsInd m o u l ->
+      ~ (annot l = Some (Some (attrName r)) /\ M.find (attrName dm) (calls l) <> None) ->
+      SubstepsInd
+        (Mod (getRegInits m)
+             (map
+                (fun newr =>
+                   if string_dec (attrName r) (attrName newr)
+                   then inlineDmToRule newr dm
+                   else newr) (getRules m)) (getDefsBodies m)) o u l.
+  Proof.
+    induction 1; intros; [constructor|].
+    subst; econstructor.
+
+    - apply IHSubstepsInd.
+      intro Hx; elim H4; clear H4; dest; split.
+      + clear -H1 H2.
+        inv H1; dest.
+        destruct l as [ann ds cs], sul as [|];
+          simpl in *; subst; intuition idtac.
+      + intro Hx; elim H3; clear H3.
+        destruct l as [ann ds cs]; simpl in *; findeq.
+
+    - instantiate (1:= scs); instantiate (1:= sul); instantiate (1:= su).
+      clear -H0 H4.
+      inv H0; try constructor.
+
+      + destruct (string_dec (attrName r) k); subst.
+        * remember (M.find (attrName dm) scs) as ods; destruct ods.
+          { elim H4; clear H4; split.
+            { destruct l as [ann ds cs]; simpl; destruct ann; reflexivity. }
+            { destruct l as [ann ds cs]; simpl.
+              rewrite M.find_union, <-Heqods; discriminate.
+            }
+          }
+          { econstructor.
+            { simpl.
+              apply in_map with (f:= fun newr =>
+                                       if string_dec (attrName r) (attrName newr)
+                                       then inlineDmToRule newr dm
+                                       else newr) in HInRules.
+              simpl in HInRules.
+              destruct (string_dec (attrName r) (attrName r)); [clear e|elim n; reflexivity].
+              eauto.
+            }
+            { simpl; destruct dm as [dmn dmb].
+              apply inlineDm_SemAction_intact; auto.
+            }
+          }
+        * econstructor.
+          { simpl.
+            apply in_map with (f:= fun newr =>
+                                     if string_dec (attrName r) (attrName newr)
+                                     then inlineDmToRule newr dm
+                                     else newr) in HInRules.
+            simpl in HInRules.
+            destruct (string_dec (attrName r) k); [elim n; auto|].
+            eauto.
+          }
+          { auto. }
+
+      + econstructor; eauto.
+
+    - auto.
+    - auto.
+    - auto.
+
+  Qed.
+
+  Lemma inlineDmToRule_substepsInd_intact_2:
+    forall o pu pds pcs,
+      SubstepsInd m o pu {| annot := None; defs := pds; calls := pcs |} ->
+      forall ru rcs,
+        Substep m o ru (Rle (Some (attrName r))) rcs ->
+        None = M.find (elt:=sigT SignT) (attrName dm) rcs ->
+        (* Some s = M.find (elt:=sigT SignT) (attrName dm) pcs -> *)
+        M.Disj ru pu -> M.Disj rcs pcs ->
+        SubstepsInd
+          (Mod (getRegInits m)
+               (map
+                  (fun newr =>
+                     if string_dec (attrName r) (attrName newr)
+                     then inlineDmToRule newr dm else newr)
+                  (getRules m)) (getDefsBodies m)) o (M.union pu ru)
+          {| annot := Some (Some (attrName r)); defs := pds; calls := M.union rcs pcs |}.
+  Proof.
+    intros; econstructor.
+
+    - apply inlineDmToRule_substepsInd_intact_1.
+      + eassumption.
+      + simpl; intro Hx; dest; discriminate.
+
+    - instantiate (1:= rcs).
+      instantiate (1:= Rle (Some (attrName r))).
+      instantiate (1:= ru).
+      inv H0.
+
+      econstructor.
+      + simpl.
+        apply in_map with (f:= fun newr =>
+                                 if string_dec (attrName r) (attrName newr)
+                                 then inlineDmToRule newr dm
+                                 else newr) in HInRules.
+        simpl in HInRules.
+        destruct (string_dec (attrName r) (attrName r)); [clear e|elim n; reflexivity].
+        eauto.
+      + simpl; destruct dm as [dmn dmb].
+        apply inlineDm_SemAction_intact; auto.
+
+    - repeat split; auto.
+    - reflexivity.
+    - reflexivity.
+
+  Qed.
+
+  Lemma inlineDmToRule_substepsInd_sub:
+    forall o u su scs s l,
+      Substep m o su (Rle (Some (attrName r))) scs ->
+      M.find (elt:=sigT SignT) (attrName dm) scs = Some s ->
+      SubstepsInd m o u l ->
+      forall ds cs,
+        l = {| annot := None; defs:= ds; calls := cs |} ->
+        M.Disj su u -> M.Disj scs cs ->
+        M.find (elt:=sigT SignT) (attrName dm) ds = Some s ->
+        SubstepsInd
+          (Mod (getRegInits m)
+               (map
+                  (fun newr =>
+                     if string_dec (attrName r) (attrName newr)
+                     then inlineDmToRule newr dm else newr)
+                  (getRules m)) (getDefsBodies m)) o (M.union u su)
+          (hideMeth 
+             {| annot := Some (Some (attrName r));
+                defs := ds;
+                calls := M.union scs cs |} (attrName dm)).
+  Proof.
+    induction 3; simpl; intros; [exfalso; inv H1; mred|].
+
+    subst; destruct l as [pann pds pcs].
+    destruct pann as [|]; [exfalso; destruct sul; inv H6|].
+    specialize (IHSubstepsInd _ _ eq_refl).
+
+    remember (M.find (attrName dm) pds) as odp; destruct odp.
+
+    - assert (s = s0); subst.
+      { clear -Heqodp H3 H6 H9.
+        inv H3; dest; simpl in *.
+        inv H6.
+        destruct sul as [|[[dmn dmb]|]]; simpl in *; findeq.
+        destruct (string_dec (attrName dm) dmn).
+        { subst; exfalso; mcontra. }
+        { mred. }
+      }
+
+      econstructor.
+      + apply IHSubstepsInd; auto.
+        inv H6; auto.
+      + instantiate (1:= scs0); instantiate (1:= sul); instantiate (1:= su0).
+        destruct sul as [|]; [exfalso; inv H6|].
+        clear -H2.
+        inv H2; [constructor|].
+        econstructor; eauto.
+      + inv H6; inv H3; dest; simpl in *.
+        unfold hideMeth; simpl.
+        rewrite <-Heqodp.
+        rewrite M.find_union, H0.
+        destruct (signIsEq _ _); [|elim n; reflexivity].
+        repeat split; simpl; auto.
+        destruct sul as [|[|]]; auto.
+        * inv H5.
+        * findeq; auto.
+      + meq.
+      + unfold hideMeth at 1; simpl.
+        rewrite H9.
+        rewrite M.find_union, H0.
+        destruct (signIsEq _ _); [clear e|elim n; reflexivity].
+        unfold hideMeth; simpl.
+        rewrite <-Heqodp.
+        rewrite M.find_union, H0.
+        destruct (signIsEq _ _); [clear e|elim n; reflexivity].
+        f_equal.
+        * inv H6; destruct sul as [|[|]]; auto; inv H5.
+        * inv H6; inv H3; dest; simpl in *.
+          destruct sul as [|[[dmn dmb]|]]; auto.
+          destruct (string_dec (attrName dm) dmn); auto.
+          subst; meq.
+          simpl in H6; mcontra.
+        * inv H6; inv H3; dest; simpl in *.
+          apply eq_sym in H0; meq.
+          
+    - clear IHSubstepsInd.
+      assert (sul = Meth (Some (attrName dm :: s)%struct)); subst.
+      { destruct sul as [|]; inv H6.
+        destruct o0 as [[dmn dmb]|]; [|mred].
+        destruct (string_dec (attrName dm) dmn); subst; mred.
+      }
+      inv H3; inv H6; dest; simpl in *; clear H5 H9.
+
+      econstructor.
+      + apply inlineDmToRule_substepsInd_intact_1.
+        * eassumption.
+        * simpl; intro Hx; dest; discriminate.
+      + instantiate (1:= M.remove (attrName dm) (M.union scs scs0)).
+        instantiate (1:= Rle (Some (attrName r))).
+        instantiate (1:= M.union su su0).
+
+        inv H; inv H2.
+        econstructor.
+        * simpl.
+          apply in_map with (f:= fun newr =>
+                                   if string_dec (attrName r) (attrName newr)
+                                   then inlineDmToRule newr dm
+                                   else newr) in HInRules.
+          simpl in HInRules.
+          destruct (string_dec _ _); [|elim n; reflexivity].
+          eauto.
+        * simpl; inv Hsig.
+          assert (dm = f) by (eapply in_NoDup_attr; eauto); subst.
+          rewrite M.union_comm with (m1:= su) by auto.
+          replace (M.remove (attrName f) (M.union scs scs0)) with
+          (M.union scs0 (M.remove (attrName f) scs))
+            by (meq; apply eq_sym in H0; mcontra).
+          eapply inlineDm_correct_SemAction; eauto.
+
+      + repeat split; auto.
+      + meq.
+      + unfold hideMeth; simpl; mred.
+        simpl; f_equal; meq.
+
+  Qed.
+
+  Lemma inlineDmToRule_wellHidden:
+    forall l,
+      wellHidden m l ->
+      wellHidden
+        (Mod (getRegInits m)
+             (map
+                (fun newr =>
+                   if string_dec (attrName r) (attrName newr)
+                   then inlineDmToRule newr dm else newr)
+                (getRules m)) (getDefsBodies m)) l.
+  Proof.
+    intros; apply wellHidden_weakening with (m2:= m); auto.
+    - unfold getCalls; simpl.
+      apply SubList_app_3; [|apply SubList_app_2, SubList_refl].
+      clear -Hdm.
+      induction (getRules m); [apply SubList_nil|].
+      apply SubList_app_3.
+      + destruct (string_dec _ _).
+        * simpl.
+          pose proof (inlineDm_calls _ _ Hdm (attrType a typeUT)).
+          apply SubList_trans with (l2:= getCallsA (attrType a typeUT)
+                                                   ++ getCallsM (getDefsBodies m)); auto.
+          apply SubList_app_3.
+          { apply SubList_app_1, SubList_app_1, SubList_refl. }
+          { apply SubList_app_2, SubList_refl. }
+        * simpl.
+          apply SubList_app_1, SubList_app_1, SubList_refl.
+      + fold getCallsR.
+        apply SubList_trans with (l2:= getCallsR l ++ getCallsM (getDefsBodies m)); auto.
+        apply SubList_app_3.
+        * apply SubList_app_1, SubList_app_2, SubList_refl.
+        * apply SubList_app_2, SubList_refl.
+    - apply SubList_refl.
+  Qed.
+
+  Lemma inlineDmToRule_stepInd:
+    forall o u l,
+      StepInd m o u l ->
+      StepInd
+        (Mod (getRegInits m)
+             (map
+                (fun newr =>
+                   if string_dec (attrName r) (attrName newr)
+                   then inlineDmToRule newr dm else newr)
+                (getRules m)) (getDefsBodies m)) o u l.
+  Proof.
+    intros; inv H.
+
+    destruct l0 as [ann ds cs].
+    assert (ann = Some (Some (attrName r)) \/ ~ ann = Some (Some (attrName r))).
+    { destruct ann; [|right; discriminate].
+      destruct o0; [|right; discriminate].
+      destruct (string_dec s (attrName r)).
+      { subst; left; reflexivity. }
+      { right; intro Hx; inv Hx; elim n; reflexivity. }
+    }
+
+    destruct H.
+
+    - subst.
+      pose proof (substepsInd_rule_split HSubSteps) as Hsp.
+      clear HSubSteps.
+      specialize (Hsp _ eq_refl).
+      destruct Hsp as [ru [rcs [pu [pl ?]]]]; dest; subst.
+
+      remember (M.find (attrName dm) rcs) as odr; destruct odr.
+
+      + rewrite <-hideMeth_preserves_hide with (dm:= attrName dm).
+        constructor.
+        * destruct pl as [pann pds pcs]; inv H3.
+          inv H1; dest; simpl in *; mred.
+          destruct pann; [inv H3|].
+          eapply inlineDmToRule_substepsInd_sub; eauto.
+
+          clear -Hdm Heqodr HWellHidden.
+          apply wellHidden_find_1 with (a:= attrName dm) in HWellHidden.
+          { simpl in *; destruct HWellHidden; mred. }
+          { apply in_map; auto. }
+          
+        * rewrite hideMeth_preserves_hide.
+          apply inlineDmToRule_wellHidden; auto.
+
+      + destruct pl as [pann pds pcs]; simpl in *.
+        remember (M.find (attrName dm) pcs) as odp; destruct odp.
+
+        * econstructor.
+          { mred; inv H3; clear H4.
+            inv H1; dest; simpl in *.
+            destruct pann; [inv H3|].
+            apply inlineDmToRule_substepsInd_intact_2; auto.
+          }
+          { apply inlineDmToRule_wellHidden; auto. }
+
+        * econstructor.
+          { apply inlineDmToRule_substepsInd_intact_1; auto.
+            { econstructor; eauto. }
+            { simpl; intro Hx; dest.
+              elim H4; clear H4.
+              inv H3; findeq.
+            }
+          }
+          { apply inlineDmToRule_wellHidden; auto. }
+
+    - econstructor.
+      + apply inlineDmToRule_substepsInd_intact_1; auto.
+        simpl; intro Hx; dest; elim H; auto.
+      + apply inlineDmToRule_wellHidden; auto.
+
+  Qed.
+
+  Lemma inlineDmToRule_traceRefines_1:
+    m <<== (Mod (getRegInits m)
+                (map (fun newr =>
+                        if string_dec (attrName r) (attrName newr)
+                        then inlineDmToRule newr dm
+                        else newr) (getRules m))
+                (getDefsBodies m)).
+  Proof.
+    apply stepRefinement with (ruleMap:= fun _ s => Some s) (theta:= id); auto.
+    intros; exists u; split; auto.
+
+    rewrite idElementwiseId.
+    replace (liftPLabel _ _ _ _) with l; [|destruct l as [[[|]|] ? ?]; simpl; f_equal].
+    unfold id.
+
+    clear H.
+    apply step_consistent; apply step_consistent in H0.
+    apply inlineDmToRule_stepInd; auto.
+  Qed.
+
+  Hypotheses (Hequiv: ModEquiv type typeUT m)
+             (HrCalls: In (attrName dm) (getCallsA (attrType r typeUT)))
+             (HnoRuleCalls: forall rule,
+                 In rule (getRules m) ->
+                 attrName rule <> attrName r ->
+                 noCallDmSigA (attrType rule typeUT)
+                              (attrName dm) (projT1 (attrType dm)) = true)
+             (HnoMethCalls: forall meth,
+                 In meth (getDefsBodies m) ->
+                 noCallDmSigA (projT2 (attrType meth) typeUT tt)
+                              (attrName dm) (projT1 (attrType dm)) = true).
+
+  Lemma getCallsA_getCalls_In:
+    In (attrName dm) (getCalls m).
+  Proof.
+    unfold getCalls.
+    apply in_or_app; left.
+    clear -Hrule HrCalls.
+    induction (getRules m); auto.
+    destruct Hrule; [subst|].
+    - simpl; apply in_or_app; left; auto.
+    - simpl; apply in_or_app; right; auto.
+  Qed.
+
+  Lemma inlineDmToRule_noDup:
+    NoDup (namesOf (getDefsBodies (Mod (getRegInits m)
+                                       (map
+                                          (fun newr =>
+                                             if string_dec (attrName r) (attrName newr)
+                                             then inlineDmToRule newr dm else newr)
+                                          (getRules m))
+                                       (getDefsBodies m)))).
+  Proof. simpl; auto. Qed.
+
+  Lemma inlineDmToRule_In:
+    In dm (getDefsBodies (Mod (getRegInits m)
+                              (map
+                                 (fun newr =>
+                                    if string_dec (attrName r) (attrName newr)
+                                    then inlineDmToRule newr dm else newr)
+                                 (getRules m))
+                              (getDefsBodies m))).
+  Proof. simpl; auto. Qed.
+
+  Lemma inlineDmToRule_ModEquiv:
+    ModEquiv type typeUT (Mod (getRegInits m)
+                              (map (fun newr =>
+                                      if string_dec (attrName r) (attrName newr)
+                                      then inlineDmToRule newr dm
+                                      else newr) (getRules m))
+                              (getDefsBodies m)).
+  Proof.
+    clear -Hequiv Hdm.
+    assert (MethEquiv type typeUT dm).
+    { inv Hequiv.
+      rewrite MethsEquiv_in in H0.
+      apply H0; auto.
+    }
+    inv Hequiv.
+    constructor; simpl; auto; clear H1.
+    induction H0; simpl; [constructor|].
+    constructor; auto.
+    destruct (string_dec _ _); auto.
+    apply inlineDm_ActionEquiv; auto.
+  Qed.
+
+  Lemma inlineDmToRule_traceRefines_2:
+    m <<== (Mod (getRegInits m)
+                (map (fun newr =>
+                        if string_dec (attrName r) (attrName newr)
+                        then inlineDmToRule newr dm
+                        else newr) (getRules m))
+                (filterDm (getDefsBodies m) (attrName dm))).
+  Proof.
+    apply stepRefinement with (ruleMap:= fun _ s => Some s) (theta:= id); auto.
+    intros; exists u; split; auto.
+
+    rewrite idElementwiseId.
+    replace (liftPLabel _ _ _ _) with l; [|destruct l as [[[|]|] ? ?]; simpl; f_equal].
+    unfold id.
+
+    clear H.
+    apply step_consistent; apply step_consistent in H0.
+
+    pose proof (inlineDmToRule_stepInd H0).
+    
+    apply stepInd_filterDm; auto.
+
+    - apply inlineDmToRule_ModEquiv.
+    - inv H0; pose proof getCallsA_getCalls_In.
+      clear -HWellHidden H0.
+      destruct (hide l0) as [ann ds cs].
+      unfold wellHidden in HWellHidden; dest; simpl in *.
+      specialize (H (attrName dm) H0).
+      findeq.
+    - constructor; simpl.
+      + apply Forall_forall; intros.
+        destruct (string_dec (attrName r) (attrName x)).
+        * apply in_map_iff in H1; dest.
+          destruct (string_dec _ _); subst; auto.
+          apply inlineDmToRule_noCallDmSigA; auto.
+        * apply HnoRuleCalls; auto.
+          apply in_map_iff in H1; dest.
+          destruct (string_dec _ _); subst; auto.
+          elim n; auto.
+      + apply Forall_forall; intros.
+        apply HnoMethCalls; auto.
+  Qed.
+
+End Partial.
 
